L3-L4 preserves observations

theories/L3_flattenedApp/instances.v
@@ -3,12 +3,10 @@ Require Import L3.wcbvEval.
 Require Import certiClasses.
 Require Import Common.Common.
 
-
-(* Do we need to use [L4.L3_to_L4_correct.eval_env]? on the environment*)
 Instance bigStepOpSemL3Term:
   BigStepOpSem (Program Term) (Program Term).
 Proof.
-  intros s sv. destruct s, sv. exact (WcbvEval env main main0 /\ env = env0).
+  intros s sv. destruct s, sv. exact (WcbvEval_env env env0 /\ WcbvEval env main main0).
 Defined.
 
 Instance WfL3Term : GoodTerm (Program L3.compile.Term) :=
@@ -16,12 +14,49 @@ Instance WfL3Term : GoodTerm (Program L3.compile.Term) :=
 
 Require Import certiClasses2.
 (* FIX!! *)
+
+Definition question_head (Q : Question) (p : Program L3.compile.Term) := 
+  match Q with
+  | Abs => match main p with
+            TLambda _ _ => true
+          | _ => false
+          end
+  | Cnstr i n =>
+    match main p with
+    | TConstruct i' n' args =>
+      if eq_dec i i' then if eq_dec n n' then true else false else false
+    | _ => false
+    end
+  end.
+(* FIX!! *)
+
 Global Instance QuestionHeadTermL : QuestionHead (Program L3.compile.Term) :=
-fun q t => false.
+  question_head.
 
 (* FIX!! *)
+
+Fixpoint tnth (n : nat) (t : Terms) :=
+  match t with
+  | tnil => None
+  | tcons t ts =>
+    match n with
+    | 0 => Some t
+    | S n => tnth n ts
+    end
+  end.
+
+Definition observe_nth_subterm (n : nat) (p : Program L3.compile.Term) := 
+  match main p with
+  | TConstruct i' n' args =>
+    match tnth n args with
+    | None => None
+    | Some t => Some {| env := env p; main := t|}
+    end
+  | _ => None
+  end.
+    
 Global Instance ObsSubtermL : ObserveNthSubterm (Program L3.compile.Term) :=
-fun n t => None.
+  observe_nth_subterm.
 
 Instance certiL3 : CerticoqLanguage (Program L3.compile.Term) := {}.
 
